imports.v
@@ -5,3 +5,11 @@ From Equations Require Export Equations.
 From Hammer Require Export Tactics.
 From stdpp Require Export relations (rtc, rtc_transitive, rtc_once, rtc_inv, rtc(..), diamond, confluent, diamond_confluent).
 Require Export Psatz.
+
+Global Set Warnings "-notation-overridden".
+From WR Require Export syntax.
+
+Notation "s [ sigmatm ]" := (subst_tm sigmatm s) (at level 7, left associativity) : subst_scope.
+Notation "s ⟨ xitm ⟩" := (ren_tm xitm s) (at level 7, left associativity) : subst_scope.
+
+Global Open Scope subst_scope. 
